add point_add

code/k256/Hacl.Impl.K256.Point.fst
@@ -14,50 +14,49 @@ open Hacl.K256.Field
 #set-options "--z3rlimit 50 --fuel 0 --ifuel 0"
 
 // (_X, _Y, _Z)
-// felem = lbuffer uint64 4ul
 inline_for_extraction noextract
-let point = lbuffer uint64 12ul
+let point = lbuffer uint64 (nlimb *! 3ul)
 
 
 inline_for_extraction noextract
 let getx (p:point) : Stack felem
   (requires fun h -> live h p)
-  (ensures fun h0 f h1 -> f == gsub p 0ul 4ul /\ h0 == h1)
-  = sub p 0ul 4ul
+  (ensures fun h0 f h1 -> f == gsub p 0ul nlimb /\ h0 == h1)
+  = sub p 0ul nlimb
 
 inline_for_extraction noextract
 let gety (p:point) : Stack felem
   (requires fun h -> live h p)
-  (ensures fun h0 f h1 -> f == gsub p 4ul 4ul /\ h0 == h1)
-  = sub p 4ul 4ul
+  (ensures fun h0 f h1 -> f == gsub p nlimb nlimb /\ h0 == h1)
+  = sub p nlimb nlimb
 
 inline_for_extraction noextract
 let getz (p:point) : Stack felem
   (requires fun h -> live h p)
-  (ensures fun h0 f h1 -> f == gsub p 8ul 4ul /\ h0 == h1)
-  = sub p 8ul 4ul
-
+  (ensures fun h0 f h1 -> f == gsub p (2ul *! nlimb) nlimb /\ h0 == h1)
+  = sub p (2ul *! nlimb) nlimb
+ 
 noextract
 let point_inv (h:mem) (p:point) =
-  fe_lt_prime h (gsub p 0ul 4ul) /\
-  fe_lt_prime h (gsub p 4ul 4ul) /\
-  fe_lt_prime h (gsub p 8ul 4ul)
+  fe_lt_prime h (gsub p 0ul nlimb) /\
+  fe_lt_prime h (gsub p nlimb nlimb) /\
+  fe_lt_prime h (gsub p (2ul *! nlimb) nlimb)
 
 
 noextract
 let point_as_nat3 (h:mem) (p:point) =
-  (as_nat h (gsub p 0ul 4ul),
-   as_nat h (gsub p 4ul 4ul),
-   as_nat h (gsub p 8ul 4ul))
+  (as_nat h (gsub p 0ul nlimb),
+   as_nat h (gsub p nlimb nlimb),
+   as_nat h (gsub p (2ul *! nlimb) nlimb))
 
 noextract
 let point_as_nat3_proj (h:mem) (p:point{point_inv h p}) : GTot Spec.K256.proj_point =
-  (as_nat h (gsub p 0ul 4ul),
-   as_nat h (gsub p 4ul 4ul),
-   as_nat h (gsub p 8ul 4ul))
+  (as_nat h (gsub p 0ul nlimb),
+   as_nat h (gsub p nlimb nlimb),
+   as_nat h (gsub p (2ul *! nlimb) nlimb))
 
 noextract
 let point_eval (h:mem) (p:point) =
-  (feval h (gsub p 0ul 4ul),
-   feval h (gsub p 4ul 4ul),
-   feval h (gsub p 8ul 4ul))
+  (feval h (gsub p 0ul nlimb),
+   feval h (gsub p nlimb nlimb),
+   feval h (gsub p (2ul *! nlimb) nlimb))
